Finish proof of simple example

src/examples/simple.v
@@ -18,6 +18,9 @@ Proof. apply _. Qed.
 Instance nat_abstract_state : AbstractState nat.
 Proof. esplit; apply _. Defined.
 
+Lemma subseteq_nat_le (n m : nat) : n ⊑ m = (n ≤ m).
+Proof. done. Qed.
+
 Definition prog : expr := let: "l" := ref #1 in ! "l".
 
 Definition pure : expr :=
@@ -76,24 +79,32 @@ Section simple_increment.
     Fence ;;
     #ℓb <- #1.
 
+  (* After a crash the following is possible: [a = 0, b = 0], [a = 1, b = 0],
+  and [a = 1, b = 1]. The case that is _not_ possible is: [a = 0, b = 1]. *)
+
   Definition recover (ℓa ℓb : loc) : expr :=
     let: "a" := ! #ℓa in
     let: "b" := ! #ℓb in
-    if: "b" ≤ "a"
+    if: "a" < "b"
     then #() #() (* Get stuck. *)
     else #().
+
+  Definition crash_condition {hD : nvmDeltaG Σ} ℓa ℓb : dProp Σ :=
+    ("pred1" ∷ ⎡ know_pred ℓa (λ (n : nat) v _, ⌜v = #n⌝) ⎤ ∗
+     "pred2" ∷ ⎡ know_pred ℓb (λ (n : nat) v hG, ⌜v = #n⌝ ∗ know_flush_lb ℓa n) ⎤ ∗
+     "pts" ∷ ∃ (sa sb : list nat), "aPts" ∷ ℓa ↦ₚ sa ∗ "bPts" ∷ ℓb ↦ₚ sb)%I.
 
   (* NOTE: This example is currently broken since the crash condition used is
   not objective. We should use the post crash modality in the crash condition
   (maybe built in to WPC). *)
-  Lemma wp_incr ℓa ℓb n E (Φ : val → dProp Σ) :
+  Lemma wp_incr ℓa ℓb s n E :
     ⊢ ⎡ know_pred ℓa (λ (n : nat) v _, ⌜v = #n⌝) ⎤ -∗
       ⎡ know_pred ℓb (λ (n : nat) v hG, ⌜v = #n⌝ ∗ know_flush_lb ℓa n) ⎤ -∗
       ℓa ↦ₚ [0] -∗
       ℓb ↦ₚ [0] -∗
-      WPC (incr_both ℓa ℓb) @ n; E
+      WPC (incr_both ℓa ℓb) @ s; n; E
         {{ λ _, ℓa ↦ₚ [0; 1] ∗ ℓb ↦ₚ [0; 1] }}
-        {{ <PC> _, ∃ (sa sb : list nat), ℓa ↦ₚ sa ∗ ℓb ↦ₚ sb }}.
+        {{ <PC> _, crash_condition ℓa ℓb }}.
   Proof.
     iIntros "#pred1 #pred2 aPts bPts".
     rewrite /incr_both.
@@ -102,11 +113,13 @@ Section simple_increment.
     wpc_bind (_ <- _)%E.
     iApply wpc_atomic_no_mask.
     iSplit. {
+      iDestruct "pred1" as "-#pred1". iDestruct "pred2" as "-#pred2".
       iCrash.
-      (* iDestruct "pred1" as "-#pred1". iDestruct "pred2" as "-#pred2". *)
-      iDestruct "aPts" as (? ?) "aPts".
-      iDestruct "bPts" as (? ?) "bPts".
-      iExists _, _. iFrame. }
+      iDestruct "aPts" as (? ?) "[aPts recA]".
+      iDestruct "bPts" as (? ?) "[bPts recB]".
+      iDestruct (recovered_at_or_lost with "recA pred1") as "pred1".
+      iDestruct (recovered_at_or_lost with "recB pred2") as "pred2".
+      iFrame. iExists _, _. iFrame. }
     iApply (wp_store_ex with "[$aPts]").
     { reflexivity. }
     { suff leq : (0 ≤ 1); first apply leq. lia. }
@@ -114,85 +127,221 @@ Section simple_increment.
     simpl.
     iNext. iIntros "aPts".
     iSplit. {
-      iModIntro. iCrash.
-      iDestruct "aPts" as (? ?) "aPts".
-      iDestruct "bPts" as (? ?) "bPts".
-      iExists _, _. iFrame. }
+      iModIntro.
+      iDestruct "pred1" as "-#pred1". iDestruct "pred2" as "-#pred2".
+      iCrash.
+      iDestruct "aPts" as (? ?) "[aPts recA]".
+      iDestruct "bPts" as (? ?) "[bPts recB]".
+      iDestruct (recovered_at_or_lost with "recA pred1") as "pred1".
+      iDestruct (recovered_at_or_lost with "recB pred2") as "pred2".
+      iFrame. iExists _, _. iFrame. }
     iModIntro.
     wpc_pures.
-    { iCrash.
-      iDestruct "aPts" as (? ?) "aPts".
-      iDestruct "bPts" as (? ?) "bPts".
-      iExists _, _. iFrame. }
+    { iDestruct "pred1" as "-#pred1". iDestruct "pred2" as "-#pred2".
+      iCrash.
+      iDestruct "aPts" as (? ?) "[aPts recA]".
+      iDestruct "bPts" as (? ?) "[bPts recB]".
+      iDestruct (recovered_at_or_lost with "recA pred1") as "pred1".
+      iDestruct (recovered_at_or_lost with "recB pred2") as "pred2".
+      iFrame. iExists _, _. iFrame. }
 
     (* The write back *)
     wpc_bind (WB _)%E.
     iApply wpc_atomic_no_mask.
     iSplit. {
+      iDestruct "pred1" as "-#pred1". iDestruct "pred2" as "-#pred2".
       iCrash.
-      iDestruct "aPts" as (? ?) "aPts".
-      iDestruct "bPts" as (? ?) "bPts".
-      iExists _, _. iFrame. }
+      iDestruct "aPts" as (? ?) "[aPts recA]".
+      iDestruct "bPts" as (? ?) "[bPts recB]".
+      iDestruct (recovered_at_or_lost with "recA pred1") as "pred1".
+      iDestruct (recovered_at_or_lost with "recB pred2") as "pred2".
+      iFrame. iExists _, _. iFrame. }
     iApply (wp_wb_ex with "aPts"); first reflexivity.
     iNext.
     iIntros "[aPts afterFence]".
     iSplit. {
       iClear "afterFence". (* FIXME: [iModIntro] spins in the absence of this. *)
-      iModIntro. iCrash.
-      iDestruct "aPts" as (? ?) "aPts".
-      iDestruct "bPts" as (? ?) "bPts".
-      iExists _, _. iFrame. }
+      iModIntro.
+      iDestruct "pred1" as "-#pred1". iDestruct "pred2" as "-#pred2".
+      iCrash.
+      iDestruct "aPts" as (? ?) "[aPts recA]".
+      iDestruct "bPts" as (? ?) "[bPts recB]".
+      iDestruct (recovered_at_or_lost with "recA pred1") as "pred1".
+      iDestruct (recovered_at_or_lost with "recB pred2") as "pred2".
+      iFrame. iExists _, _. iFrame. }
     iModIntro.
     wpc_pures.
     { iClear "afterFence". (* FIXME: [iModIntro] spins in the absence of this. *)
+      iDestruct "pred1" as "-#pred1". iDestruct "pred2" as "-#pred2".
       iCrash.
-      iDestruct "aPts" as (? ?) "aPts".
-      iDestruct "bPts" as (? ?) "bPts".
-      iExists _, _. iFrame. }
+      iDestruct "aPts" as (? ?) "[aPts recA]".
+      iDestruct "bPts" as (? ?) "[bPts recB]".
+      iDestruct (recovered_at_or_lost with "recA pred1") as "pred1".
+      iDestruct (recovered_at_or_lost with "recB pred2") as "pred2".
+      iFrame. iExists _, _. iFrame. }
 
     (* The fence. *)
     wpc_bind (Fence)%E.
     iApply wpc_atomic_no_mask.
     iSplit. {
       iClear "afterFence". (* FIXME: [iModIntro] spins in the absence of this. *)
+      iDestruct "pred1" as "-#pred1". iDestruct "pred2" as "-#pred2".
       iCrash.
-      iDestruct "aPts" as (? ?) "aPts".
-      iDestruct "bPts" as (? ?) "bPts".
-      iExists _, _. iFrame. }
+      iDestruct "aPts" as (? ?) "[aPts recA]".
+      iDestruct "bPts" as (? ?) "[bPts recB]".
+      iDestruct (recovered_at_or_lost with "recA pred1") as "pred1".
+      iDestruct (recovered_at_or_lost with "recB pred2") as "pred2".
+      iFrame. iExists _, _. iFrame. }
     iApply (wp_fence with "afterFence").
     iNext.
     iIntros "#pLowerBound".
     iSplit. {
-      iModIntro. iCrash.
-      iDestruct "aPts" as (? ?) "aPts".
-      iDestruct "bPts" as (? ?) "bPts".
-      iExists _, _. iFrame. }
+      iModIntro.
+      iDestruct "pred1" as "-#pred1". iDestruct "pred2" as "-#pred2".
+      iCrash.
+      iDestruct "aPts" as (? ?) "[aPts recA]".
+      iDestruct "bPts" as (? ?) "[bPts recB]".
+      iDestruct (recovered_at_or_lost with "recA pred1") as "pred1".
+      iDestruct (recovered_at_or_lost with "recB pred2") as "pred2".
+      iFrame. iExists _, _. iFrame. }
     iModIntro.
     wpc_pures.
-    { iCrash.
-      iDestruct "aPts" as (? ?) "aPts".
-      iDestruct "bPts" as (? ?) "bPts".
-      iExists _, _. iFrame. }
+    {
+      iDestruct "pred1" as "-#pred1". iDestruct "pred2" as "-#pred2".
+      iCrash.
+      iDestruct "aPts" as (? ?) "[aPts recA]".
+      iDestruct "bPts" as (? ?) "[bPts recB]".
+      iDestruct (recovered_at_or_lost with "recA pred1") as "pred1".
+      iDestruct (recovered_at_or_lost with "recB pred2") as "pred2".
+      iFrame. iExists _, _. iFrame. }
 
     (* The last store *)
     iApply wpc_atomic_no_mask.
     iSplit.
-    { iCrash.
-      iDestruct "aPts" as (? ?) "aPts".
-      iDestruct "bPts" as (? ?) "bPts".
-      iExists _, _. iFrame. }
+    { iDestruct "pred1" as "-#pred1". iDestruct "pred2" as "-#pred2".
+      iCrash.
+      iDestruct "aPts" as (? ?) "[aPts recA]".
+      iDestruct "bPts" as (? ?) "[bPts recB]".
+      iDestruct (recovered_at_or_lost with "recA pred1") as "pred1".
+      iDestruct (recovered_at_or_lost with "recB pred2") as "pred2".
+      iFrame. iExists _, _. iFrame. }
     iApply (wp_store_ex with "[$bPts]").
     { reflexivity. }
     { suff leq : (0 ≤ 1); first apply leq. lia. }
     { iFrame "#". iFrame "pLowerBound". done. }
     iNext. iIntros "bPts".
     iSplit. {
-      iModIntro. iCrash.
-      iDestruct "aPts" as (? ?) "aPts".
-      iDestruct "bPts" as (? ?) "bPts".
-      iExists _, _. iFrame. }
+      iModIntro.
+      iDestruct "pred1" as "-#pred1". iDestruct "pred2" as "-#pred2".
+      iCrash.
+      iDestruct "aPts" as (? ?) "[aPts recA]".
+      iDestruct "bPts" as (? ?) "[bPts recB]".
+      iDestruct (recovered_at_or_lost with "recA pred1") as "pred1".
+      iDestruct (recovered_at_or_lost with "recB pred2") as "pred2".
+      iFrame. iExists _, _. iFrame. }
     iModIntro.
     iFrame "aPts bPts".
+  Qed.
+
+  Lemma wpc_recover `{hD : nvmDeltaG Σ} ℓa ℓb s k E :
+    crash_condition ℓa ℓb -∗
+    WPC recover ℓa ℓb
+      @ s; k; E
+      {{ _, True }}
+      {{ <PC> H0, crash_condition ℓa ℓb }}.
+  Proof.
+    iNamed 1. iNamed "pts".
+    rewrite /recover.
+    iDestruct (mapsto_ex_last with "aPts") as %[sA saEq].
+    iDestruct (mapsto_ex_last with "bPts") as %[sB sbEq].
+
+    (* Load [ℓa]. *)
+    wpc_bind (! _)%E.
+    iApply wpc_atomic_no_mask.
+    iSplit. {
+      iDestruct "pred1" as "-#pred1". iDestruct "pred2" as "-#pred2".
+      iCrash.
+      iDestruct "aPts" as (? ?) "[aPts recA]".
+      iDestruct "bPts" as (? ?) "[bPts recB]".
+      iDestruct (recovered_at_or_lost with "recA pred1") as "pred1".
+      iDestruct (recovered_at_or_lost with "recB pred2") as "pred2".
+      iFrame. iExists _, _. iFrame. }
+    iDestruct "pred1" as "#pred1".
+    iDestruct "pred2" as "#pred2".
+    iApply (wp_load_ex _ _ _ _ (λ v, ⌜v = #sA⌝)%I with "[$aPts $pred1]"); first done.
+    { iModIntro. naive_solver. }
+    iIntros "!>" (?) "[aPts ->]".
+    iSplit.
+    { iModIntro.
+      iDestruct "pred1" as "-#pred1". iDestruct "pred2" as "-#pred2".
+      iCrash.
+      iDestruct "aPts" as (? ?) "[aPts recA]".
+      iDestruct "bPts" as (? ?) "[bPts recB]".
+      iDestruct (recovered_at_or_lost with "recA pred1") as "pred1".
+      iDestruct (recovered_at_or_lost with "recB pred2") as "pred2".
+      iFrame. iExists _, _. iFrame. }
+
+    iModIntro.
+    wpc_pures.
+    { iDestruct "pred1" as "-#pred1". iDestruct "pred2" as "-#pred2".
+      iCrash.
+      iDestruct "aPts" as (? ?) "[aPts recA]".
+      iDestruct "bPts" as (? ?) "[bPts recB]".
+      iDestruct (recovered_at_or_lost with "recA pred1") as "pred1".
+      iDestruct (recovered_at_or_lost with "recB pred2") as "pred2".
+      iFrame. iExists _, _. iFrame. }
+
+    (* Load [ℓb]. *)
+    wpc_bind (! _)%E.
+    iApply wpc_atomic_no_mask.
+    iSplit. {
+      iDestruct "pred1" as "-#pred1". iDestruct "pred2" as "-#pred2".
+      iCrash.
+      iDestruct "aPts" as (? ?) "[aPts recA]".
+      iDestruct "bPts" as (? ?) "[bPts recB]".
+      iDestruct (recovered_at_or_lost with "recA pred1") as "pred1".
+      iDestruct (recovered_at_or_lost with "recB pred2") as "pred2".
+      iFrame. iExists _, _. iFrame. }
+    iDestruct "pred1" as "#pred1".
+    iDestruct "pred2" as "#pred2".
+    iApply (wp_load_ex _ _ _ _ (λ v, ⌜v = #sB⌝ ∗ know_flush_lb ℓa sB)%I
+              with "[$bPts $pred2]"); first done.
+    { iModIntro. iIntros (?) "[-> hi]". naive_solver. }
+    iIntros "!>" (?) "(bPts & -> & lub)".
+    iSplit.
+    { iModIntro.
+      iDestruct "pred1" as "-#pred1". iDestruct "pred2" as "-#pred2".
+      iCrash.
+      iDestruct "aPts" as (? ?) "[aPts recA]".
+      iDestruct "bPts" as (? ?) "[bPts recB]".
+      iDestruct (recovered_at_or_lost with "recA pred1") as "pred1".
+      iDestruct (recovered_at_or_lost with "recB pred2") as "pred2".
+      iFrame. iExists _, _. iFrame. }
+
+    iModIntro.
+    wpc_pures.
+    { iDestruct "pred1" as "-#pred1". iDestruct "pred2" as "-#pred2".
+      iCrash.
+      iDestruct "aPts" as (? ?) "[aPts recA]".
+      iDestruct "bPts" as (? ?) "[bPts recB]".
+      iDestruct (recovered_at_or_lost with "recA pred1") as "pred1".
+      iDestruct (recovered_at_or_lost with "recB pred2") as "pred2".
+      iFrame. iExists _, _. iFrame. }
+
+    iDestruct (mapsto_ex_flush_lb_incl with "lub aPts") as %incl; first done.
+    rewrite bool_decide_eq_false_2.
+    2: { rewrite subseteq_nat_le in incl. lia. }
+
+    wpc_pures.
+    { iDestruct "pred1" as "-#pred1". iDestruct "pred2" as "-#pred2".
+      iCrash.
+      iDestruct "aPts" as (? ?) "[aPts recA]".
+      iDestruct "bPts" as (? ?) "[bPts recB]".
+      iDestruct (recovered_at_or_lost with "recA pred1") as "pred1".
+      iDestruct (recovered_at_or_lost with "recB pred2") as "pred2".
+      iFrame. iExists _, _. iFrame. }
+
+    iModIntro. done.
   Qed.
 
   (* FIXME: Hoare triples don't work as Perennial's Hoare triples are tied to iProp. *)
@@ -208,8 +357,21 @@ Section simple_increment.
   (*   {{{ (True : dProp Σ) }}}. *)
 
   Lemma incr_safe s k E ℓa ℓb :
-    ⊢ wpr s k E (incr_both ℓa ℓb) (recover ℓa ℓb) (λ _, True%I) (λ _ _, True%I).
+    ⊢ ⎡ know_pred ℓa (λ (n : nat) v _, ⌜v = #n⌝) ⎤ -∗
+      ⎡ know_pred ℓb (λ (n : nat) v hG, ⌜v = #n⌝ ∗ know_flush_lb ℓa n) ⎤ -∗
+      ℓa ↦ₚ [0] -∗
+      ℓb ↦ₚ [0] -∗
+      wpr s k E (incr_both ℓa ℓb) (recover ℓa ℓb)
+        (λ _, ℓa ↦ₚ [0; 1] ∗ ℓb ↦ₚ [0; 1]) (λ _ _, True%I).
   Proof.
-  Abort.
+    iIntros "a b c d".
+    iApply (idempotence_wpr _ _ _ _ _ _ _ (λ _, <PC> _, crash_condition ℓa ℓb)%I with "[a b c d] []").
+    { iApply (wp_incr _ _ s k E with "a b c d"). }
+    do 2 iModIntro.
+    iIntros (hG') "R".
+    iNext.
+    iCrash.
+    iApply (wpc_recover with "R").
+  Qed.
 
 End simple_increment.
